

Lecture → 18Method of Variation of Parameters

$$\boxed{f(D)y = x(x)}$$

→ R.H.S will be
little bit complicated

• $\tan x$, $\ln x$, x^{-1} , e^{x^2} , ...

for a second order equation:

$$y'' + Py' + Qy = R(x).$$

1. → y_1, y_2 .

2. Assume:

$$y = u(x)y_1 + v(x)y_2.$$

3. Solve.

$$u'y_1 + v'y_2 = 0$$

$$u'y_1' + v'y_2' = R(x)$$

4. find u', v' .

5. Final solution:

5) Final solution:

$$y = uy_1 + vy_2 + \underline{\underline{CF}}$$

Examples:

#1. $y'' - y = e^x$

C.F

Auxiliary eqⁿ:

$$m^2 - 1 = 0 \quad \text{C.F} = \underline{\underline{c_1 e^x + c_2 e^{-x}}}$$

$$\Rightarrow m = \pm 1$$

$$y_1 = \underline{e^x}, \quad y_2 = e^{-x}$$

Assume: $y = ue^x + ve^{-x}$

Equations:

$$u' e^x + v' e^{-x} = 0 \quad \dots \textcircled{i}$$

$$u' e^x - v' e^{-x} = e^x \quad \dots \textcircled{ii}$$

$$2u' e^x = e^x$$

$$\Rightarrow u' = \frac{1}{2} \quad \dots \textcircled{iii}$$

$$v' = -\frac{1}{2} e^{2x} \quad \dots \textcircled{iv}$$

Integrate u' and v'

Integrate u and v

$$\left. \begin{aligned} u &= x/2 \\ v &= -\frac{1}{4} e^{2x} \end{aligned} \right\}.$$

$$y = \frac{x}{2} e^x - \frac{1}{4} e^{2x} (e^{-x})$$

$$= \frac{x}{2} e^x - \frac{1}{4} e^x$$

$$y = c_1 e^x + c_2 e^{-x} + \frac{x}{2} e^x - \frac{1}{4} e^x$$

Solution

#2 Solve:

$$\underline{y'' + y = \tan x}$$

Step 1:

$$\text{c.f. } m^2 + 1 = 0.$$

$$\Rightarrow m = \pm i.$$

$$y_1 = \cos x, \quad y_2 = \sin x.$$

$$\text{c.f.} = c_1 \cos x + c_2 \sin x.$$

Step 2:

$$y = u \cos x + v \sin x.$$

Step 3:

$$u' \cos x + v' \sin x = 0 \quad \text{--- (1)}$$

$$-u' \sin x + v' \cos x = \tan x \quad \text{--- (2)}$$

$$-u' \sin x + v' \cos x = \tan x \quad (2)$$

$$\underline{\text{eq (1)} \times \sin x} \quad \parallel \quad \underline{\text{eq (2)} \times \cos x}$$

$$\left. \begin{aligned} u' &= -\tan x \sin x = -\frac{\sin^2 x}{\cos x} \\ v' &= \tan x \cos x = \sin x \end{aligned} \right\}$$

Integrate u' and v' .

$$\frac{du}{dx} = -\frac{\sin^2 x}{\cos x}$$

$$\Rightarrow du = -\frac{\sin^2 x}{\cos x} dx$$

$$\Rightarrow du = -\left(\frac{1 - \cos^2 x}{\cos x}\right) dx$$

$$\Rightarrow du = -(sec x - \cos x) dx$$

$$\Rightarrow \int du = -\int (sec x - \cos x) dx$$

$$\Rightarrow u = -(\ln |sec x + \tan x| - \sin x)$$

$$v = -\cos x$$

Final:

$$\boxed{y = C.F + y}$$

Simultaneous Linear Differential equation.

$$\frac{dx}{dt} = ax + by$$

$$\frac{dx}{dt} = ax + by$$

$$\frac{dy}{dt} = cx + dy$$

Writing in a operator form $D = \frac{d}{dt}$

$$Dx = ax + by$$

$$\Rightarrow (D - a)x - by = 0 \quad \text{--- (i)}$$

$$-cx + (D - d)y = 0 \quad \text{--- (ii)}$$

Examples

#1. $\frac{dx}{dt} = x + y$

$$\frac{dy}{dt} = x - y$$

Writing in a operator form —

$$Dx = x + y$$

$$\Rightarrow (D - 1)x - y = 0 \quad \text{--- (i)}$$

$$Dy + y - x = 0$$

$$\Rightarrow -x + (D + 1)y = 0 \quad \text{--- (ii)}$$

$$(D^2 - 1)x - (D + 1)y = 0$$

$$-x + (D + 1)y = 0$$

$$(D^2 - 1 - 1)x = 0$$

$$\Rightarrow (D^2 - 2)x = 0$$

Auxiliary eqⁿ for m -

$$m^2 - 2 = 0$$

$$\Rightarrow m = \pm \sqrt{2}$$

$$x = c_1 e^{\sqrt{2}t} + c_2 e^{-\sqrt{2}t}$$

From eq (i) —

$$(D+1)y = x.$$

$$\Rightarrow y = x - Dy.$$

$$\Rightarrow \frac{dy}{dt} + y = x.$$

$$\Rightarrow \frac{dy}{dt} + y = c_1 e^{\sqrt{2}t} + c_2 e^{-\sqrt{2}t}$$

$$I.f = e^{\int 1 dt} = e^t$$

$$e^t \frac{dy}{dt} + e^t y = c_1 e^{(\sqrt{2}+1)t} + c_2 e^{(-\sqrt{2}+1)t}$$

$$\Rightarrow \frac{d}{dt}(y e^t) = c_1 e^{(\sqrt{2}+1)t} + c_2 e^{(-\sqrt{2}+1)t}$$

$$\Rightarrow y e^t = \frac{c_1}{\sqrt{2}+1} e^{(\sqrt{2}+1)t} + \frac{c_2}{(-\sqrt{2}+1)} e^{(-\sqrt{2}+1)t}$$

$$\Rightarrow y = \frac{c_1}{\sqrt{2}+1} e^{\sqrt{2}t} + \frac{c_2}{(-\sqrt{2}+1)} e^{-\sqrt{2}t}$$

$$\Rightarrow y = \frac{c_1}{\sqrt{2}+1} e^{\sqrt{2}t} + \frac{c_2}{1-\sqrt{2}} e^{-\sqrt{2}t}$$

$$(D+1)y = x.$$

$$\Rightarrow y = \frac{1}{D+1} x.$$

$$y = e^{-t} \int x e^t dt$$

$$(D+a)y = f(t)$$

$$\Rightarrow y = e^{-at} \int f(t) e^{at} dt.$$

Solve :

$$\left. \begin{aligned} \frac{dx}{dt} &= 3x + 4y \\ \frac{dy}{dt} &= -4x + 3y \end{aligned} \right\}$$

Step 1:

$$D = \frac{d}{dt}$$

$$\begin{aligned} (D-3)x - 4y &= 0 & - \textcircled{i} \\ 4x + (D-3)y &= 0 & - \textcircled{ii} \end{aligned}$$

Eliminate y.

$$(D-3)^2 x + 16x = 0$$

1 2. - 1 2. n

$$(D-3)x + 16x = 0$$

$$\Rightarrow (D^2 - 6D + 25)x = 0.$$

Auxiliary eqⁿ:

$$m^2 - 6m + 25 = 0.$$

$$m = \frac{6 \pm \sqrt{(-6)^2 - 4(1)(25)}}{2 \cdot 1}$$

$$= \frac{6 \pm \sqrt{36 - 100}}{2}$$

$$= \frac{6 \pm 8i}{2}$$

$$= \underline{\underline{3 \pm 4i}} \rightarrow \text{a + ib}.$$

$$x = e^{3t} (\underline{\underline{c_1 \cos 4t + c_2 \sin 4t}}).$$

$$4x + (D-3)y = 0.$$

$$\Rightarrow (D-3)y = -4x.$$

$$\Rightarrow y = \frac{1}{(D-3)} (-4x)$$

$$= \underline{\underline{e^{3t} \int (-4x) e^{-3t} dt}}$$

$$y = \dots$$

Euler - Cauchy (Equidimensional)
Differential equation

Differential eq

D.E of the form :

$$x^n \frac{d^n y}{dx^n} + a_1 x^{n-1} \frac{d^{n-1} y}{dx^{n-1}} + \dots + a_{n-1} x \frac{dy}{dx} + a_n y = 0.$$

— (1)

let assume : $y = x^m$.

Successive differentiation :

$$\frac{dy}{dx} = m x^{m-1}$$

$$\frac{d^2 y}{dx^2} = m(m-1) x^{m-2},$$

$$\frac{d^3 y}{dx^3} = m(m-1)(m-2) x^{m-3}$$

Examples :

Solve : $x^2 \frac{d^2 y}{dx^2} + x \frac{dy}{dx} - y = 0.$

→ This is an Euler-Cauchy eqⁿ

Assume : $y = x^m$.

$$\frac{dy}{dx} = m x^{m-1}$$

$$d^2 y = m(m-1) x^{m-2}.$$

$$\frac{d^2 y}{dx^2} = m(m-1)x^{m-2}$$

$$x^2 [m(m-1)x^{m-2}] + x(mx^{m-1}) - x^m = 0$$

$$\Rightarrow m(m-1)x^m + mx^m - x^m = 0$$

$$\Rightarrow x^m [m(m-1) + m - 1] = 0$$

$$\Rightarrow x^m [m^2 - 1] = 0$$

Solving the auxiliary eqⁿ:

$$m^2 - 1 = 0$$

$$\Rightarrow m = \pm 1$$

$$y = c_1 x + c_2 x^{-1}$$

Based on auxiliary eqⁿ roots:

Roots	Solution
<u>Real & distinct</u>	$y = C_1 x^{m_1} + C_2 x^{m_2}$
<u>Equal roots</u>	$y = C_1 x^m + C_2 x^m \ln x$
<u>Complex roots $m = \alpha \pm i\beta$</u>	$y = x^\alpha [C_1 \cos(\beta \ln x) + C_2 \sin(\beta \ln x)]$

H/W

Solve!

$$\left. \begin{array}{l} \text{i) } x^2 y'' - 3xy' + 4y = 0 \\ \text{ii) } x^2 y'' + xy' + y = 0 \end{array} \right\}$$

Condition for exactness of Higher order Linear differential equations

General form:

$$a_0(x) \frac{d^n y}{dx^n} + a_1(x) \frac{d^{n-1} y}{dx^{n-1}} + \dots + a_n(x) y = q(x)$$

$$\rightarrow a_0 y^n + a_1 y^{(n-1)} + \dots + a_n y = \phi(x)$$

$$\frac{d}{dx} [b_0(x) y^{n-1} + b_1(x) y^{(n-2)} + \dots + b_{n-1}(x) y] = \phi(x)$$

Expanding we get:

$$b_0 y^n + b_0' y^{n-1} + \dots + b_0 y^n + (b_0' + b_1) y^{(n-1)} + \dots + (b_1' + b_2) y^{n-2} + \dots + b_{n-1}' y$$

Comparing it with this eqⁿ:

$$a_0 y^n + a_1 y^{(n-1)} + \dots + a_n y = \phi(x)$$

$$a_0 = b_0$$

$$a_1 = b_0' + b_1$$

$$a_2 = b_1' + b_2$$

⋮

$$a_n = b'_{n-1}$$

$$a_1 = \frac{d a_0}{dx}, \quad a_2 = \frac{d a_1}{dx}$$

$$a_3 = \frac{d a_2}{dx}, \dots, a_n = \frac{d a_{n-1}}{dx}$$

$$\underline{\underline{a_k = \frac{d}{dx} (a_{k-1})}}$$

$$\# \quad x^2 y'' + 2xy' + 2y = 0 \quad \checkmark$$

$$a_0 = x^2$$

$$a_1 = 2x = \frac{d}{dx} (x^2) = a_0'$$

$$a_2 = 2 = \frac{d}{dx} (2x)$$

$$\frac{d}{dx} (x^2 y' + 2xy) = 0$$

$$x^2 y' + 2xy = \underline{C_1}$$

$$\Rightarrow x^2 \frac{dy}{dx} + 2xy = \underline{C_1}$$

$$\Rightarrow \frac{dy}{dx} + \frac{2}{x} y = \frac{C_1}{x^2}$$

$$\int \frac{2}{x} dx = x^2$$

$$I.F = e^{\int 2/x dx} = x^2.$$

$$\frac{d}{dx} (x^2 y) = c_1$$

$$\Rightarrow x^2 y = c_1 x + c_2.$$

$$\Rightarrow y = \frac{c_1}{x} + \frac{c_2}{x^2}$$

Ans

$$\left. \begin{array}{l} \textcircled{1} (1+x^2)y'' + 2xy' + 2y = 1. \\ \textcircled{2} (1+x)^2 y'' + 2(1+x)y' + 2y = 0 \end{array} \right\}$$